{
  "@context": {
    "jsonld": "http://www.w3.org/ns/json-ld#",
    "owl": "http://www.w3.org/2002/07/owl#",
    "rdf": "http://www.w3.org/1999/02/22-rdf-syntax-ns#",
    "rdfs": "http://www.w3.org/2000/01/rdf-schema#",
    "schema": "http://schema.org/",
    "xsd": "http://www.w3.org/2001/XMLSchema#",
    "Context": {
      "@id": "jsonld:Context"
    },
    "PrefixDefinition": {
      "@id": "jsonld:PrefixDefinition"
    },
    "TermDefinition": {
      "@id": "jsonld:TermDefinition"
    },
    "base": {
      "@id": "jsonld:base",
      "@type": "@id"
    },
    "container": {
      "@id": "jsonld:container",
      "@type": "@id"
    },
    "context": {
      "@id": "jsonld:context",
      "@type": "@id"
    },
    "definition": {
      "@id": "jsonld:definition",
      "@type": "@id"
    },
    "direction": {
      "@id": "jsonld:direction",
      "@language": null
    },
    "id": {
      "@id": "jsonld:id",
      "@type": "@id"
    },
    "import": {
      "@id": "jsonld:import",
      "@type": "@id"
    },
    "language": {
      "@id": "jsonld:language",
      "@language": null
    },
    "nest": {
      "@id": "jsonld:nest",
      "@language": null
    },
    "prefix": {
      "@id": "jsonld:prefix",
      "@type": "xsd:boolean"
    },
    "propagate": {
      "@id": "jsonld:propagate",
      "@type": "xsd:boolean"
    },
    "protected": {
      "@id": "jsonld:protected",
      "@type": "xsd:boolean"
    },
    "reverse": {
      "@id": "jsonld:reverse",
      "@type": "xsd:anyUri"
    },
    "term": {
      "@id": "jsonld:term",
      "@language": null
    },
    "type": {
      "@id": "jsonld:type",
      "@type": "@id"
    },
    "version": {
      "@id": "jsonld:version",
      "@type": "xsd:decimal"
    },
    "vocab": {
      "@id": "jsonld:vocab",
      "@type": "@id"
    },
    "compacted": {
      "@id": "jsonld:compacted"
    },
    "expanded": {
      "@id": "jsonld:expanded"
    },
    "flattened": {
      "@id": "jsonld:flattened"
    },
    "frame": {
      "@id": "jsonld:frame"
    },
    "framed": {
      "@id": "jsonld:framed"
    },
    "graphContainerType": {
      "@id": "jsonld:graphContainerType"
    },
    "idContainerType": {
      "@id": "jsonld:idContainerType"
    },
    "indexContainerType": {
      "@id": "jsonld:indexContainerType"
    },
    "languageContainerType": {
      "@id": "jsonld:languageContainerType"
    },
    "listContainerType": {
      "@id": "jsonld:listContainerType"
    },
    "setContainerType": {
      "@id": "jsonld:setContainerType"
    },
    "typeContainerType": {
      "@id": "jsonld:typeContainerType"
    }
  },
  "@graph": {
    "@context": {
      "id": "@id",
      "type": "@type",
      "dc": "http://purl.org/dc/terms/",
      "owl": "http://www.w3.org/2002/07/owl#",
      "rdf": "http://www.w3.org/1999/02/22-rdf-syntax-ns#",
      "rdfs": "http://www.w3.org/2000/01/rdf-schema#",
      "dc:title": {
        "@container": "@language"
      },
      "dc:description": {
        "@container": "@language"
      },
      "dc:date": {
        "@type": "xsd:date"
      },
      "rdfs:comment": {
        "@container": "@language"
      },
      "rdfs:domain": {
        "@type": "@id"
      },
      "rdfs:label": {
        "@container": "@language"
      },
      "rdfs:range": {
        "@type": "@id"
      },
      "rdfs:seeAlso": {
        "@type": "@id"
      },
      "rdfs:subClassOf": {
        "@type": "@id"
      },
      "rdfs:subPropertyOf": {
        "@type": "@id"
      },
      "owl:imports": {
        "@type": "@id"
      },
      "owl:versionInfo": {
        "@type": "@id"
      },
      "schema:domainIncludes": {
        "@type": "@vocab",
        "@container": "@set"
      },
      "schema:rangeIncludes": {
        "@type": "@vocab",
        "@container": "@set"
      },
      "rdfs_classes": {
        "@reverse": "rdfs:isDefinedBy",
        "@type": "@id"
      },
      "rdfs_properties": {
        "@reverse": "rdfs:isDefinedBy",
        "@type": "@id"
      },
      "rdfs_datatypes": {
        "@reverse": "rdfs:isDefinedBy",
        "@type": "@id"
      },
      "rdfs_instances": {
        "@reverse": "rdfs:isDefinedBy",
        "@type": "@id"
      }
    },
    "@id": "http://www.w3.org/ns/json-ld#",
    "@type": "owl:Ontology",
    "dc:title": {
      "en": "The JSON-LD Vocabulary"
    },
    "dc:description": {
      "en": "This is a vocabulary document and is used to achieve certain features of the JSON-LD language."
    },
    "dc:date": "2020-01-03",
    "owl:versionInfo": "https://github.com/w3c/json-ld-wg/commit/606458561d3761dad00912b4ac7b1959302ef304",
    "rdfs:seeAlso": [
      "http://www.w3.org/TR/json-ld11"
    ],
    "rdfs_classes": [
      {
        "@id": "jsonld:Context",
        "@type": [
          "rdfs:Class"
        ],
        "rdfs:label": {
          "en": "Context"
        },
        "rdfs:comment": {
          "en": "Defines term definitions and other aspects of a JSON-LD `Context`.\n\nA [context definition](https://www.w3.org/TR/json-ld11/#dfn-context-definition) MUST be a map whose keys MUST be either _terms_, _compact IRIs_, _IRIs_, or one of the keywords `@base`, `@import`, `@language`, `@propagate`, `@protected`, `@type`, `@version`, or `@vocab`."
        },
        "rdfs:seeAlso": "https://www.w3.org/TR/json-ld11/#context-definitions"
      },
      {
        "@id": "jsonld:PrefixDefinition",
        "@type": [
          "rdfs:Class"
        ],
        "rdfs:label": {
          "en": "Prefix Definition"
        },
        "rdfs:comment": {
          "en": "A string ([simple term definition](http://www.w3.org/TR/json-ld11/#dfn-simple-term-definitions)), expanding to an IRI."
        },
        "rdfs:seeAlso": "https://www.w3.org/TR/json-ld11/#dfn-term-definition"
      },
      {
        "@id": "jsonld:TermDefinition",
        "@type": [
          "rdfs:Class"
        ],
        "rdfs:label": {
          "en": "Term Definition"
        },
        "rdfs:comment": {
          "en": "A [term definition](http://www.w3.org/TR/json-ld11/#dfn-term-definitions) is an entry in a [context](#Context), where the key defines a term which may be used within a dictionary as a key, type, or elsewhere that a string is interpreted as a vocabulary item. Its value is an [expanded term definition](https://www.w3.org/TR/json-ld11/#dfn-expanded-term-definitions).\n\n\n\nAn [expanded term definition](https://www.w3.org/TR/json-ld11/#dfn-expanded-term-definition) MUST be a map composed of zero or more keys from `@id`, `@reverse`, `@type`, `@language`, `@container`, `@context`, `@prefix`, `@propagate`, or `@protected`. An expanded term definition SHOULD NOT contain any other keys."
        },
        "rdfs:seeAlso": "https://www.w3.org/TR/json-ld11/#dfn-term-definition"
      }
    ],
    "rdfs_properties": [
      {
        "@id": "jsonld:base",
        "@type": [
          "rdf:Property"
        ],
        "rdfs:label": {
          "en": "base"
        },
        "rdfs:comment": {
          "en": "If the [context definition](https://www.w3.org/TR/json-ld11/#dfn-context-definition) has an `@base` key, its value MUST be an _IRI reference_, or `null`."
        },
        "rdfs:seeAlso": "https://www.w3.org/TR/json-ld11/#context-definitions",
        "schema:domainIncludes": "jsonld:Context",
        "schema:rangeIncludes": "xsd:anyUri"
      },
      {
        "@id": "jsonld:container",
        "@type": [
          "rdf:Property"
        ],
        "rdfs:label": {
          "en": "container"
        },
        "rdfs:comment": {
          "en": "The associated `@container` value in an [expanded term definition](https://www.w3.org/TR/json-ld11/#dfn-expanded-term-definitions).\n\nIf the [expanded term definition](https://www.w3.org/TR/json-ld11/#dfn-expanded-term-definitions) contains the `@container` keyword, its value MUST be either `@list`, `@set`, `@language`, `@index`, `@id`, `@graph`, `@type`, or be `null` or an array containing exactly any one of those keywords, or a combination of `@set` and any of `@index`, `@id`, `@graph`, `@type`, `@language` in any order.\n\n`@container` may also be an array containing `@graph` along with either `@id` or `@index` and also optionally including `@set`.\n\nIf the value is `@language`, when the term is used outside of the `@context`, the associated value MUST be a language map.\n\nIf the value is `@index`, when the term is used outside of the `@context`, the associated value MUST be an index map."
        },
        "rdfs:seeAlso": "https://www.w3.org/TR/json-ld11/#expanded-term-definition",
        "schema:domainIncludes": "jsonld:TermDefinition",
        "schema:rangeIncludes": "jsonld:ContainerType"
      },
      {
        "@id": "jsonld:context",
        "@type": [
          "rdf:Property"
        ],
        "rdfs:label": {
          "en": "context"
        },
        "rdfs:comment": {
          "en": "As an IRI, this link relation is used to associate a JSON-LD context with a JSON document so that it can be interpreted as JSON-LD. In an HTTP request header, specifies the location of a context to use for compaction. As a Context, defines an inline `context definition`."
        },
        "rdfs:seeAlso": "https://www.w3.org/TR/json-ld11/#interpreting-json-as-json-ld",
        "schema:rangeIncludes": [
          "jsonld:Context",
          "xsd:anyUri"
        ]
      },
      {
        "@id": "jsonld:definition",
        "@type": [
          "rdf:Property"
        ],
        "rdfs:label": {
          "en": "definition"
        },
        "rdfs:comment": {
          "en": "Term definition(s) associated with this context."
        },
        "schema:domainIncludes": "jsonld:Context",
        "schema:rangeIncludes": [
          "jsonld:TermDefinition",
          "jsonld:PrefixDefinition"
        ]
      },
      {
        "@id": "jsonld:direction",
        "@type": [
          "rdf:Property"
        ],
        "rdfs:label": {
          "en": "direction"
        },
        "rdfs:comment": {
          "en": "If the [context definition](https://www.w3.org/TR/json-ld11/#dfn-context-definition) has an `@direction` key, its value MUST be one of `\"ltr\"` or `\"rtl\"`, or be `null`."
        },
        "rdfs:seeAlso": "https://www.w3.org/TR/json-ld11/#context-definitions",
        "schema:domainIncludes": [
          "jsonld:Context",
          "jsonld:TermDefinition"
        ],
        "schema:rangeIncludes": "xsd:string"
      },
      {
        "@id": "jsonld:id",
        "@type": [
          "rdf:Property"
        ],
        "rdfs:label": {
          "en": "id"
        },
        "rdfs:comment": {
          "en": "The `@id` mapping of a [term definition](#TermDefinition)."
        },
        "rdfs:seeAlso": "https://www.w3.org/TR/json-ld11/#expanded-term-definition",
        "schema:domainIncludes": [
          "jsonld:TermDefinition",
          "jsonld:PrefixDefinition"
        ],
        "schema:rangeIncludes": "xsd:anyUri"
      },
      {
        "@id": "jsonld:import",
        "@type": [
          "rdf:Property"
        ],
        "rdfs:label": {
          "en": "import"
        },
        "rdfs:comment": {
          "en": "If the [context definition](https://www.w3.org/TR/json-ld11/#dfn-context-definition) contains the `@import` keyword, its value MUST be an _IRI reference_. When used as a reference from an `@import`, the referenced context definition MUST NOT include an `@import` key, itself."
        },
        "rdfs:seeAlso": "https://www.w3.org/TR/json-ld11/#context-definitions",
        "schema:domainIncludes": "jsonld:Context",
        "schema:rangeIncludes": "xsd:anyUri"
      },
      {
        "@id": "jsonld:language",
        "@type": [
          "rdf:Property"
        ],
        "rdfs:label": {
          "en": "language"
        },
        "rdfs:comment": {
          "en": "The [default language](https://www.w3.org/TR/json-ld11/#dfn-default-language) is set in the context using the `@language` key whose value MUST be a string representing a [BCP47](https://tools.ietf.org/html/bcp47) language code or null."
        },
        "rdfs:seeAlso": "https://www.w3.org/TR/json-ld11/#dfn-default-language",
        "schema:domainIncludes": [
          "jsonld:Context",
          "jsonld:TermDefinition"
        ],
        "schema:rangeIncludes": "xsd:string"
      },
      {
        "@id": "jsonld:nest",
        "@type": [
          "rdf:Property"
        ],
        "rdfs:label": {
          "en": "nest"
        },
        "rdfs:comment": {
          "en": "If the [expanded term definition](https://www.w3.org/TR/json-ld11/#dfn-expanded-term-definitions) contains the `@nest` keyword, its value MUST be either `@nest`, or a _term_ which expands to `@nest`."
        },
        "rdfs:seeAlso": "https://www.w3.org/TR/json-ld11/#expanded-term-definition",
        "schema:domainIncludes": "jsonld:TermDefinition",
        "schema:rangeIncludes": "xsd:string"
      },
      {
        "@id": "jsonld:prefix",
        "@type": [
          "rdf:Property"
        ],
        "rdfs:label": {
          "en": "prefix"
        },
        "rdfs:comment": {
          "en": "With the value `true`, allows this term to be used to construct a compact IRI when compacting."
        },
        "rdfs:seeAlso": "https://www.w3.org/TR/json-ld11/#expanded-term-definition",
        "schema:domainIncludes": "jsonld:TermDefinition",
        "schema:rangeIncludes": "xsd:boolean"
      },
      {
        "@id": "jsonld:propagate",
        "@type": [
          "rdf:Property"
        ],
        "rdfs:label": {
          "en": "propagate"
        },
        "rdfs:comment": {
          "en": "If the [context definition](https://www.w3.org/TR/json-ld11/#dfn-context-definition) contains the `@propagate` keyword, its value MUST be `true` or `false`."
        },
        "rdfs:seeAlso": "https://www.w3.org/TR/json-ld11/#context-definitions",
        "schema:domainIncludes": [
          "jsonld:Context",
          "jsonld:TermDefinition"
        ],
        "schema:rangeIncludes": "xsd:boolean"
      },
      {
        "@id": "jsonld:protected",
        "@type": [
          "rdf:Property"
        ],
        "rdfs:label": {
          "en": "protected"
        },
        "rdfs:comment": {
          "en": "If the [context definition](https://www.w3.org/TR/json-ld11/#dfn-context-definition) contains the `@protected` keyword, its value MUST be `true` or `false`."
        },
        "rdfs:seeAlso": "https://www.w3.org/TR/json-ld11/#context-definitions",
        "schema:domainIncludes": [
          "jsonld:Context",
          "jsonld:TermDefinition"
        ],
        "schema:rangeIncludes": "xsd:boolean"
      },
      {
        "@id": "jsonld:reverse",
        "@type": [
          "rdf:Property"
        ],
        "rdfs:label": {
          "en": "reverse"
        },
        "rdfs:comment": {
          "en": "The `@reverse` mapping of an [expanded term definition](https://www.w3.org/TR/json-ld11/#dfn-expanded-term-definitions)."
        },
        "rdfs:seeAlso": "https://www.w3.org/TR/json-ld11/#expanded-term-definition",
        "schema:domainIncludes": "jsonld:TermDefinition",
        "schema:rangeIncludes": "xsd:anyUri"
      },
      {
        "@id": "jsonld:term",
        "@type": [
          "rdf:Property"
        ],
        "rdfs:label": {
          "en": "term"
        },
        "rdfs:comment": {
          "en": "The term associated with a [term definition](#TermDefinition)."
        },
        "rdfs:seeAlso": "https://www.w3.org/TR/json-ld11/#dfn-term",
        "schema:domainIncludes": [
          "jsonld:TermDefinition",
          "jsonld:PrefixDefinition"
        ],
        "schema:rangeIncludes": "xsd:string"
      },
      {
        "@id": "jsonld:type",
        "@type": [
          "rdf:Property"
        ],
        "rdfs:label": {
          "en": "type"
        },
        "rdfs:comment": {
          "en": "If the [context definition](https://www.w3.org/TR/json-ld11/#dfn-context-definition) contains the `@type` keyword, its value MUST be a map with only the entry `@container` set to `@set`, and optionally an entry `@protected`.\n\n\n\nIf the [expanded term definition](https://www.w3.org/TR/json-ld11/#dfn-expanded-term-definitions) contains the `@type` keyword, its value MUST be an _IRI reference_, a _term_, `null`, or one of the keywords `@id`, `@json`, `@none`, or `@vocab`."
        },
        "rdfs:seeAlso": "https://www.w3.org/TR/json-ld11/#context-definitions",
        "schema:domainIncludes": [
          "jsonld:Context",
          "jsonld:TermDefinition"
        ],
        "schema:rangeIncludes": [
          "xsd:anyUri",
          "xsd:string"
        ]
      },
      {
        "@id": "jsonld:version",
        "@type": [
          "rdf:Property"
        ],
        "rdfs:label": {
          "en": "version"
        },
        "rdfs:comment": {
          "en": "The [processing mode](https://www.w3.org/TR/json-ld11/#dfn-processing-mode) defines how a JSON-LD document is processed. By default, all documents are assumed to be conformant with [JSON-LD 1.1`](http://www.w3.org/TR/json-ld11). By defining a different version via explicit API option, other processing modes can be accessed. This specification defines extensions for the `json-ld-1.1` processing mode."
        },
        "rdfs:seeAlso": "https://www.w3.org/TR/json-ld11/#dfn-processing-mode",
        "schema:domainIncludes": "jsonld:Context",
        "schema:rangeIncludes": "xsd:decimal"
      },
      {
        "@id": "jsonld:vocab",
        "@type": [
          "rdf:Property"
        ],
        "rdfs:label": {
          "en": "vocab"
        },
        "rdfs:comment": {
          "en": "Used to expand properties and values in `@type` with a common prefix IRI."
        },
        "rdfs:seeAlso": "https://www.w3.org/TR/json-ld11/#default-vocabulary",
        "schema:domainIncludes": "jsonld:Context",
        "schema:rangeIncludes": "xsd:anyUri"
      }
    ],
    "rdfs_instances": [
      {
        "@id": "jsonld:compacted",
        "@type": [
          "owl:NamedIndividual"
        ],
        "rdfs:label": {
          "en": "compacted"
        },
        "rdfs:comment": {
          "en": "This profile IRI is used to request or specify compacted JSON-LD document form."
        },
        "rdfs:seeAlso": "https://www.w3.org/TR/json-ld11/#iana-considerations"
      },
      {
        "@id": "jsonld:expanded",
        "@type": [
          "owl:NamedIndividual"
        ],
        "rdfs:label": {
          "en": "expanded"
        },
        "rdfs:comment": {
          "en": "This profile URI is used to request or specify expanded JSON-LD document form."
        },
        "rdfs:seeAlso": "https://www.w3.org/TR/json-ld11/#iana-considerations"
      },
      {
        "@id": "jsonld:flattened",
        "@type": [
          "owl:NamedIndividual"
        ],
        "rdfs:label": {
          "en": "flattened"
        },
        "rdfs:comment": {
          "en": "This profile URI is used to request or specify flattened JSON-LD document form."
        },
        "rdfs:seeAlso": "https://www.w3.org/TR/json-ld11/#iana-considerations"
      },
      {
        "@id": "jsonld:frame",
        "@type": [
          "owl:NamedIndividual"
        ],
        "rdfs:label": {
          "en": "frame"
        },
        "rdfs:comment": {
          "en": "As an IRI, this link relation is used to associate a JSON-LD frame with a JSON-LD document. In an HTTP request header, specifies the location of a frame to use for framing."
        },
        "rdfs:seeAlso": "https://www.w3.org/TR/json-ld11/#iana-considerations"
      },
      {
        "@id": "jsonld:framed",
        "@type": [
          "owl:NamedIndividual"
        ],
        "rdfs:label": {
          "en": "framed"
        },
        "rdfs:comment": {
          "en": "This profile URI is used to request or specify framed JSON-LD document form."
        },
        "rdfs:seeAlso": "https://www.w3.org/TR/json-ld11/#iana-considerations"
      },
      {
        "@id": "jsonld:graphContainerType",
        "@type": [
          "ContainerType"
        ],
        "rdfs:label": {
          "en": "@graph"
        },
        "rdfs:comment": {
          "en": "If the [expanded term definition](https://www.w3.org/TR/json-ld11/#dfn-expanded-term-definitions) contains the `@container` keyword, its value MUST be either `@list`, `@set`, `@language`, `@index`, `@id`, `@graph`, `@type`, or be `null` or an _array_ containing exactly any one of those keywords."
        },
        "rdfs:seeAlso": "https://www.w3.org/TR/json-ld11/#context-definitions"
      },
      {
        "@id": "jsonld:idContainerType",
        "@type": [
          "ContainerType"
        ],
        "rdfs:label": {
          "en": "@id"
        },
        "rdfs:comment": {
          "en": "If the [expanded term definition](https://www.w3.org/TR/json-ld11/#dfn-expanded-term-definitions) contains the `@container` keyword, its value MUST be either `@list`, `@set`, `@language`, `@index`, `@id`, `@graph`, `@type`, or be `null` or an _array_ containing exactly any one of those keywords."
        },
        "rdfs:seeAlso": "https://www.w3.org/TR/json-ld11/#context-definitions"
      },
      {
        "@id": "jsonld:indexContainerType",
        "@type": [
          "ContainerType"
        ],
        "rdfs:label": {
          "en": "@index"
        },
        "rdfs:comment": {
          "en": "If the [expanded term definition](https://www.w3.org/TR/json-ld11/#dfn-expanded-term-definitions) contains the `@container` keyword, its value MUST be either `@list`, `@set`, `@language`, `@index`, `@id`, `@graph`, `@type`, or be `null` or an _array_ containing exactly any one of those keywords."
        },
        "rdfs:seeAlso": "https://www.w3.org/TR/json-ld11/#context-definitions"
      },
      {
        "@id": "jsonld:languageContainerType",
        "@type": [
          "ContainerType"
        ],
        "rdfs:label": {
          "en": "@language"
        },
        "rdfs:comment": {
          "en": "If the [expanded term definition](https://www.w3.org/TR/json-ld11/#dfn-expanded-term-definitions) contains the `@container` keyword, its value MUST be either `@list`, `@set`, `@language`, `@index`, `@id`, `@graph`, `@type`, or be `null` or an _array_ containing exactly any one of those keywords."
        },
        "rdfs:seeAlso": "https://www.w3.org/TR/json-ld11/#context-definitions"
      },
      {
        "@id": "jsonld:listContainerType",
        "@type": [
          "ContainerType"
        ],
        "rdfs:label": {
          "en": "@list"
        },
        "rdfs:comment": {
          "en": "If the [expanded term definition](https://www.w3.org/TR/json-ld11/#dfn-expanded-term-definitions) contains the `@container` keyword, its value MUST be either `@list`, `@set`, `@language`, `@index`, `@id`, `@graph`, `@type`, or be `null` or an _array_ containing exactly any one of those keywords."
        },
        "rdfs:seeAlso": "https://www.w3.org/TR/json-ld11/#context-definitions"
      },
      {
        "@id": "jsonld:setContainerType",
        "@type": [
          "ContainerType"
        ],
        "rdfs:label": {
          "en": "@set"
        },
        "rdfs:comment": {
          "en": "If the [expanded term definition](https://www.w3.org/TR/json-ld11/#dfn-expanded-term-definitions) contains the `@container` keyword, its value MUST be either `@list`, `@set`, `@language`, `@index`, `@id`, `@graph`, `@type`, or be `null` or an _array_ containing exactly any one of those keywords."
        },
        "rdfs:seeAlso": "https://www.w3.org/TR/json-ld11/#context-definitions"
      },
      {
        "@id": "jsonld:typeContainerType",
        "@type": [
          "ContainerType"
        ],
        "rdfs:label": {
          "en": "@type"
        },
        "rdfs:comment": {
          "en": "If the [expanded term definition](https://www.w3.org/TR/json-ld11/#dfn-expanded-term-definitions) contains the `@container` keyword, its value MUST be either `@list`, `@set`, `@language`, `@index`, `@id`, `@graph`, `@type`, or be `null` or an _array_ containing exactly any one of those keywords."
        },
        "rdfs:seeAlso": "https://www.w3.org/TR/json-ld11/#context-definitions"
      }
    ]
  }
}
